Finish the easy half of the DRF with several admits left.

src/drf/PromiseIndep.v
@@ -17,14 +17,148 @@ Require Import Progress.
 
 Set Implicit Arguments.
 
+Definition ThreadEvent_is_promising (e: ThreadEvent.t) : option (Loc.t * Time.t) :=
+  match e with
+  | ThreadEvent.promise loc from to v rel => Some (loc, to)
+  | _ => None
+  end.
 
 Inductive small_step (e:ThreadEvent.t) (tid:Ident.t) (c1:Configuration.t): forall (c2:Configuration.t), Prop :=
 | small_step_intro
-    lang st1 lc1 st2 lc2 memory2
+    lang st1 st2 lc1 lc2 sc2 memory2
     (TID: IdentMap.find tid c1.(Configuration.threads) = Some (existT _ lang st1, lc1))
-    (STEP: Thread.step e (Thread.mk _ st1 lc1 c1.(Configuration.memory)) (Thread.mk _ st2 lc2 memory2)):
-    small_step e tid c1 (Configuration.mk (IdentMap.add tid (existT _ _ st2, lc2) c1.(Configuration.threads)) memory2)
+    (STEP: Thread.step e (Thread.mk _ st1 lc1 c1.(Configuration.sc) c1.(Configuration.memory)) (Thread.mk _ st2 lc2 sc2 memory2)):
+    small_step e tid c1 (Configuration.mk (IdentMap.add tid (existT _ _ st2, lc2) c1.(Configuration.threads)) sc2 memory2)
 .
+
+Inductive tau_small_step (tid:Ident.t) (c1 c2:Configuration.t): Prop :=
+| tau_small_step_intro
+    e
+    (STEP: small_step e tid c1 c2)
+    (TAU: ThreadEvent.get_event e = None)
+.
+
+Inductive small_step_all (tid:Ident.t) (c1 c2:Configuration.t): Prop :=
+| small_step_all_intro e
+    (STEP: small_step e tid c1 c2)
+.
+
+Inductive pf_step (e:ThreadEvent.t) (tid:Ident.t) (c1:Configuration.t): forall (c2:Configuration.t), Prop :=
+| pf_step_intro c2
+    (STEP: small_step e tid c1 c2)
+    (NO_PROMISE: ThreadEvent_is_promising e = None):
+    pf_step e tid c1 c2
+.
+
+Inductive pf_step_all (c1 c2:Configuration.t): Prop :=
+| pf_step_all_intro
+    e tid
+    (PI_STEP: pf_step e tid c1 c2)
+.
+
+(* NOTE: `race_rw` requires two *distinct* threads to have a race.
+ * However, C/C++ acknowledges intra-thread races.  For example,
+ * according to the Standard, `f(x=1, x)` is RW-racy on `x`, since the
+ * order of evaluation of the arguments is unspecified.  We currently
+ * ignore this aspect of the race semantics.
+ *)
+
+Inductive race_condition e1 e2 ord1 ord2 : Prop :=
+| race_condition_rw loc
+    (EVENT1: ProgramEvent.is_reading e1 = Some (loc, ord1))
+    (EVENT2: ProgramEvent.is_writing e2 = Some (loc, ord2))
+| race_condition_ww loc
+    (EVENT1: ProgramEvent.is_writing e1 = Some (loc, ord1))
+    (EVENT2: ProgramEvent.is_writing e2 = Some (loc, ord2))
+.
+Hint Constructors race_condition.
+
+Inductive race (c:Configuration.t) (ord1 ord2:Ordering.t): Prop :=
+| race_intro
+    tid1 lang1 st1 lc1 e1 st1'
+    tid2 lang2 st2 lc2 e2 st2'
+    (TID: tid1 <> tid2)
+    (TH1: IdentMap.find tid1 c.(Configuration.threads) = Some (existT _ lang1 st1, lc1))
+    (TH2: IdentMap.find tid2 c.(Configuration.threads) = Some (existT _ lang2 st2, lc2))
+    (STATE1: lang1.(Language.step) (Some e1) st1 st1')
+    (STATE2: lang2.(Language.step) (Some e2) st2 st2')
+    (EVENT: race_condition e1 e2 ord1 ord2)
+.              
+
+Definition pf_racefree (c1:Configuration.t): Prop :=
+  forall c2 ordr ordw
+    (STEPS: rtc pf_step_all c1 c2)
+    (RACE: race c2 ordr ordw),
+    <<ORDR: Ordering.le Ordering.acqrel ordr>> /\
+    <<ORDW: Ordering.le Ordering.acqrel ordw>>.
+
+Inductive pi_step: Ident.t -> Configuration.t*Configuration.t -> Configuration.t*Configuration.t -> Prop :=
+| pi_step_step
+    e tid cS1 cT1 cS2 cT2
+    (STEPT: small_step e tid cT1 cT2)
+    (STEPS: if ThreadEvent_is_promising e
+            then cS1 = cS2
+            else small_step e tid cS1 cS2)
+    (LANGMATCH: 
+     option_map fst (IdentMap.find tid cS2.(Configuration.threads)) =
+     option_map fst (IdentMap.find tid cT2.(Configuration.threads))):
+  pi_step tid (cS1,cT1) (cS2,cT2)
+.
+
+Inductive pi_step_except (tid_except:Ident.t) cST1 cST2: Prop :=
+| pi_step_except_intro
+    tid
+    (PI_STEP: pi_step tid cST1 cST2)
+    (TID: tid <> tid_except)
+.
+
+Inductive pi_step_all cST1 cST2: Prop :=
+| pi_step_all_intro
+    tid
+    (PI_STEP: pi_step tid cST1 cST2)
+.
+
+Definition Threads_remove_promise (ths: Threads.t) : Threads.t :=
+  IdentMap.map
+  (fun th => (th.(fst), Local.mk th.(snd).(Local.commit) Memory.bot))
+  ths.
+
+Inductive pi_wf: Configuration.t*Configuration.t -> Prop :=
+| pi_wf_intro sc mS mT thsS thsT
+    (THS: thsS = Threads_remove_promise thsT)
+    (WFT: Configuration.wf (Configuration.mk thsT sc mT))
+    (WFS: Configuration.wf (Configuration.mk thsS sc mS))
+    (LR: forall loc ts from msg
+           (IN: Memory.get loc ts mS = Some (from, msg)),
+         <<IN: Memory.get loc ts mT = Some (from, msg)>> /\
+         <<NOT: forall tid, ~Threads.is_promised tid loc ts thsT>>)
+    (RL: forall loc ts from msg
+           (IN: Memory.get loc ts mT = Some (from, msg))
+           (NOT: forall tid, ~Threads.is_promised tid loc ts thsT),
+         Memory.get loc ts mS = Some (from, msg)):
+  pi_wf (Configuration.mk thsS sc mS, Configuration.mk thsT sc mT)
+.
+
+Inductive pi_consistent: Configuration.t*Configuration.t -> Prop :=
+| pi_consistent_intro cS1 cT1
+  (CONSIS:
+    forall tid cS2 cT2 lst2 lc2 loc ts from msg
+    (* (TID: IdentMap.find tid cT1.(Configuration.threads) <> None) *)
+    (STEPS: rtc (pi_step_except tid) (cS1,cT1) (cS2,cT2))
+    (THREAD: IdentMap.find tid cT2.(Configuration.threads) = Some (lst2, lc2))
+    (PROMISE: Memory.get loc ts lc2.(Local.promises) = Some (from, msg)),
+  exists cS3 cT3 lst3 lc3,
+    <<STEPS: rtc (pi_step tid) (cS2,cT2) (cS3,cT3)>> /\
+    <<THREAD: IdentMap.find tid cT3.(Configuration.threads) = Some (lst3, lc3)>> /\
+    <<PROMISE: Memory.get loc ts lc3.(Local.promises) = None>>):
+  pi_consistent (cS1, cT1).
+
+Definition pi_racefree (cST1:Configuration.t*Configuration.t): Prop :=
+  forall cST2 ordr ordw
+    (STEPS: rtc pi_step_all cST1 cST2)
+    (RACE: race (fst cST2) ordr ordw),
+    <<ORDR: Ordering.le Ordering.acqrel ordr>> /\
+    <<ORDW: Ordering.le Ordering.acqrel ordw>>.
 
 Lemma small_step_future
       e tid c1 c2
@@ -33,10 +167,10 @@ Lemma small_step_future
   <<WF2: Configuration.wf c2>> /\
   <<FUTURE: Memory.future c1.(Configuration.memory) c2.(Configuration.memory)>>.
 Proof.
-  inv WF1. inv WF. inv STEP.
+  inv WF1. inv WF. inv STEP. ss.
   exploit THREADS; ss; eauto. i.
-  exploit Thread.step_future; eauto. s. i. des.
-  splits; [|by eauto]. econs; ss. econs.
+  exploit Thread.step_future; eauto.
+  s; i; des. splits; [|by eauto]. econs; ss. econs.
   - i. Configuration.simplify.
     + congr.
     + exploit THREADS; try apply TH1; eauto. i. des.
@@ -52,34 +186,27 @@ Proof.
     auto.
 Qed.
 
-Inductive tau_small_step (tid:Ident.t) (c1 c2:Configuration.t): Prop :=
-| tau_small_step_intro
-    e
-    (STEP: small_step e tid c1 c2)
-    (TAU: ThreadEvent.get_event e = None)
-.
-
 Lemma thread_step_small_step
       lang e tid threads
-      st1 lc1 mem1
-      st2 lc2 mem2
+      st1 lc1 sc1 mem1
+      st2 lc2 sc2 mem2
       (TID: IdentMap.find tid threads = Some (existT _ lang st1, lc1))
-      (STEP: Thread.step e (Thread.mk lang st1 lc1 mem1) (Thread.mk lang st2 lc2 mem2)):
+      (STEP: Thread.step e (Thread.mk lang st1 lc1 sc1 mem1) (Thread.mk lang st2 lc2 sc2 mem2)):
   small_step e tid
-             (Configuration.mk threads mem1)
-             (Configuration.mk (IdentMap.add tid (existT _ lang st2, lc2) threads) mem2).
+             (Configuration.mk threads sc1 mem1)
+             (Configuration.mk (IdentMap.add tid (existT _ lang st2, lc2) threads) sc2 mem2).
 Proof.
   econs; eauto.
 Qed.
 
 Lemma thread_step_small_step_aux
       lang e tid threads
-      st1 lc1 mem1
-      st2 lc2 mem2
-      (STEP: Thread.step e (Thread.mk lang st1 lc1 mem1) (Thread.mk lang st2 lc2 mem2)):
+      st1 lc1 sc1 mem1
+      st2 lc2 sc2 mem2
+      (STEP: Thread.step e (Thread.mk lang st1 lc1 sc1 mem1) (Thread.mk lang st2 lc2 sc2 mem2)):
   small_step e tid
-             (Configuration.mk (IdentMap.add tid (existT _ lang st1, lc1) threads) mem1)
-             (Configuration.mk (IdentMap.add tid (existT _ lang st2, lc2) threads) mem2).
+             (Configuration.mk (IdentMap.add tid (existT _ lang st1, lc1) threads) sc1 mem1)
+             (Configuration.mk (IdentMap.add tid (existT _ lang st2, lc2) threads) sc2 mem2).
 Proof.
   exploit thread_step_small_step; eauto.
   { eapply IdentMap.Facts.add_eq_o. eauto. }
@@ -92,8 +219,8 @@ Lemma rtc_tau_thread_step_rtc_tau_small_step_aux
       (TID: IdentMap.find tid threads = Some (existT _ lang th1.(Thread.state), th1.(Thread.local)))
       (STEP: (rtc (@Thread.tau_step lang)) th1 th2):
   rtc (tau_small_step tid)
-      (Configuration.mk threads th1.(Thread.memory))
-      (Configuration.mk (IdentMap.add tid (existT _ lang th2.(Thread.state), th2.(Thread.local)) threads) th2.(Thread.memory)).
+      (Configuration.mk threads th1.(Thread.sc) th1.(Thread.memory))
+      (Configuration.mk (IdentMap.add tid (existT _ lang th2.(Thread.state), th2.(Thread.local)) threads) th2.(Thread.sc) th2.(Thread.memory)).
 Proof.
   revert threads TID. induction STEP; i.
   - apply rtc_refl. f_equal. apply IdentMap.eq_leibniz. ii.
@@ -108,13 +235,13 @@ Qed.
 
 Lemma rtc_tau_thread_step_rtc_tau_small_step
       lang tid threads
-      st1 lc1 mem1
-      st2 lc2 mem2
+      st1 lc1 sc1 mem1
+      st2 lc2 sc2 mem2
       (TID: IdentMap.find tid threads = Some (existT _ lang st1, lc1))
-      (STEP: (rtc (@Thread.tau_step lang)) (Thread.mk lang st1 lc1 mem1) (Thread.mk lang st2 lc2 mem2)):
+      (STEP: (rtc (@Thread.tau_step lang)) (Thread.mk lang st1 lc1 sc1 mem1) (Thread.mk lang st2 lc2 sc2 mem2)):
   rtc (tau_small_step tid)
-      (Configuration.mk threads mem1)
-      (Configuration.mk (IdentMap.add tid (existT _ lang st2, lc2) threads) mem2).
+      (Configuration.mk threads sc1 mem1)
+      (Configuration.mk (IdentMap.add tid (existT _ lang st2, lc2) threads) sc2 mem2).
 Proof.
   exploit rtc_tau_thread_step_rtc_tau_small_step_aux; eauto. auto.
 Qed.
@@ -137,119 +264,111 @@ Proof.
   - eapply thread_step_small_step_aux. eauto.
 Qed.
 
-Definition pi_machine_event (e:ThreadEvent.t) (threads:Threads.t): Prop :=
-  match ThreadEvent.is_reading e with
-  | Some (loc, ts, _) => ~ Threads.is_promised loc ts threads
-  | None => True
-  end.
-
-Inductive pi_step (tid:Ident.t) (c1 c2:Configuration.t): Prop :=
-| pi_step_intro
-    e
-    (STEP: small_step e tid c1 c2)
-    (READINFO: pi_machine_event e c1.(Configuration.threads))
-.
-
 Lemma pi_step_future
-      tid c1 c2
-      (WF1: Configuration.wf c1)
-      (STEP: pi_step tid c1 c2):
-  <<WF2: Configuration.wf c2>> /\
-  <<FUTURE: Memory.future c1.(Configuration.memory) c2.(Configuration.memory)>>.
-Proof. inv STEP. eapply small_step_future; eauto. Qed.
+      tid cST1 cST2
+      (WF1: pi_wf cST1)
+      (STEP: pi_step tid cST1 cST2):
+  <<WF2: pi_wf cST2>> /\
+  <<FUTURES: Memory.future cST1.(fst).(Configuration.memory) cST2.(fst).(Configuration.memory)>> /\
+  <<FUTURET: Memory.future cST1.(snd).(Configuration.memory) cST2.(snd).(Configuration.memory)>>.
+Proof.
+  inv WF1. inv STEP. splits; cycle 1. 
+  - destruct (ThreadEvent_is_promising e).
+    + subst. ss. econs.
+    + eapply small_step_future in STEPS; eauto; des; ss.
+  - eapply small_step_future in STEPT; eauto; des; ss.
+  - assert (WFT2: Configuration.wf cT2).
+    { by eapply small_step_future, STEPT. }
+    assert (WFS2: Configuration.wf cS2).
+    { destruct (ThreadEvent_is_promising e); [by inv STEPS|].
+      by eapply small_step_future, STEPS. }
+    inv STEPT. inv STEP; inv STEP0; ss.
+    { subst. inv LOCAL. econs; eauto.
+      - apply IdentMap.eq_leibniz.
+        ii. setoid_rewrite IdentMap.map_add.
+        destruct (Loc.eq_dec y tid) eqn: TIDEQ.
+        + subst. setoid_rewrite IdentMap.Properties.F.map_o.
+          rewrite IdentMap.gss, TID. done.
+        + by rewrite IdentMap.gso.
+      - admit.
+      - admit.
+    }
+    { inv STEPS. inv STEP; inv STEP0; try done. econs; eauto; ss.
+      - apply IdentMap.eq_leibniz. ii.
+        setoid_rewrite IdentMap.Properties.F.map_o in TID0.
+        rewrite TID in TID0. inv TID0. depdes H1.
+        setoid_rewrite IdentMap.map_add.
+        rewrite !IdentMap.gss in LANGMATCH. depdes LANGMATCH.
+        destruct (Loc.eq_dec y tid) eqn: TIDEQ.
+        + subst. by rewrite !IdentMap.gss.
+        + by rewrite !IdentMap.gso.
+      - admit.
+      - admit.
+    }
+    { admit. }
+    { admit. }
+    { admit. }
+    { admit. }
+    { admit. }
+Admitted.
 
 Lemma rtc_pi_step_future
-      tid c1 c2
-      (WF1: Configuration.wf c1)
-      (STEPS: rtc (pi_step tid) c1 c2):
-  <<WF2: Configuration.wf c2>> /\
-  <<FUTURE: Memory.future c1.(Configuration.memory) c2.(Configuration.memory)>>.
+      tid cST1 cST2
+      (WF1: pi_wf cST1)
+      (STEPS: rtc (pi_step tid) cST1 cST2):
+  <<WF2: pi_wf cST2>> /\
+  <<FUTURES: Memory.future cST1.(fst).(Configuration.memory) cST2.(fst).(Configuration.memory)>> /\
+  <<FUTURET: Memory.future cST1.(snd).(Configuration.memory) cST2.(snd).(Configuration.memory)>>.
 Proof.
   revert WF1. induction STEPS; i.
-  - splits; auto. refl.
+  - splits; auto; econs.
   - exploit pi_step_future; eauto. i. des.
     exploit IHSTEPS; eauto. i. des.
-    splits; auto. etrans; eauto.
+    splits; auto; etrans; eauto.
 Qed.
 
-Inductive pi_step_all (c1 c2:Configuration.t): Prop :=
-| pi_step_all_intro
-    tid
-    (PI_STEP: pi_step tid c1 c2)
-.
-
-Inductive pi_step_except (tid_except:Ident.t) (c1 c2:Configuration.t): Prop :=
-| pi_step_except_intro
-    tid
-    (PI_STEP: pi_step tid c1 c2)
-    (TID: tid <> tid_except)
-.
-
-Definition pi_consistent (c1:Configuration.t): Prop :=
-  forall tid c2
-    (TID: IdentMap.find tid c1.(Configuration.threads) <> None)
-    (STEPS: rtc (pi_step_except tid) c1 c2),
-  exists c3 lang st3 lc3,
-    <<STEPS: rtc (pi_step tid) c2 c3>> /\
-    <<THREAD: IdentMap.find tid c3.(Configuration.threads) = Some (existT _ lang st3, lc3)>> /\
-    <<PROMISES: lc3.(Local.promises) = Memory.bot>>.
-
 Lemma pi_step_find
-      tid1 tid2 c1 c2
-      (STEP: pi_step tid1 c1 c2)
+      tid1 tid2 cST1 cST2
+      (STEP: pi_step tid1 cST1 cST2)
       (TID: tid1 <> tid2):
-  IdentMap.find tid2 c2.(Configuration.threads) = IdentMap.find tid2 c1.(Configuration.threads).
+  IdentMap.find tid2 cST2.(fst).(Configuration.threads) = IdentMap.find tid2 cST1.(fst).(Configuration.threads) /\
+  IdentMap.find tid2 cST2.(snd).(Configuration.threads) = IdentMap.find tid2 cST1.(snd).(Configuration.threads).
 Proof.
-  inv STEP. inv STEP0. s. rewrite IdentMap.Facts.add_neq_o; auto.
+  inv STEP; split; cycle 1.
+  - inv STEPT. s. erewrite IdentMap.Facts.add_neq_o; eauto.
+  - destruct (ThreadEvent_is_promising e).
+    + subst. econs; auto.
+    + depdes STEPS. s. erewrite IdentMap.Facts.add_neq_o; eauto.
 Qed.
 
 Lemma rtc_pi_step_find
-      tid1 tid2 c1 c2
-      (STEP: rtc (pi_step tid1) c1 c2)
+      tid1 tid2 cST1 cST2
+      (STEP: rtc (pi_step tid1) cST1 cST2)
       (TID: tid1 <> tid2):
-  IdentMap.find tid2 c2.(Configuration.threads) = IdentMap.find tid2 c1.(Configuration.threads).
+  IdentMap.find tid2 cST2.(snd).(Configuration.threads) = IdentMap.find tid2 cST1.(snd).(Configuration.threads).
 Proof.
-  induction STEP; auto. erewrite IHSTEP, pi_step_find; eauto.
+  induction STEP; auto. 
+  des. erewrite IHSTEP.
+  eapply pi_step_find; eauto.
 Qed.
 
-(* NOTE: `race_rw` requires two *distinct* threads to have a race.
- * However, C/C++ acknowledges intra-thread races.  For example,
- * according to the Standard, `f(x=1, x)` is RW-racy on `x`, since the
- * order of evaluation of the arguments is unspecified.  We currently
- * ignore this aspect of the race semantics.
- *)
-Inductive race_rw (c:Configuration.t) (ordr ordw:Ordering.t): Prop :=
-| race_rw_intro
-    tid1 lang1 st1 lc1 e1 st1'
-    tid2 lang2 st2 lc2 e2 st2'
-    loc
-    (TID: tid1 <> tid2)
-    (TH1: IdentMap.find tid1 c.(Configuration.threads) = Some (existT _ lang1 st1, lc1))
-    (TH2: IdentMap.find tid2 c.(Configuration.threads) = Some (existT _ lang2 st2, lc2))
-    (STATE1: lang1.(Language.step) (Some e1) st1 st1')
-    (STATE2: lang2.(Language.step) (Some e2) st2 st2')
-    (EVENT1: ProgramEvent.is_reading e1 = Some (loc, ordr))
-    (EVENT2: ProgramEvent.is_writing e2 = Some (loc, ordw))
-.
-
-Definition pi_racefree (c1:Configuration.t): Prop :=
-  forall c2 ordr ordw
-    (STEPS: rtc pi_step_all c1 c2)
-    (RACE: race_rw c2 ordr ordw),
-    <<ORDR: Ordering.le Ordering.acqrel ordr>> /\
-    <<ORDW: Ordering.le Ordering.acqrel ordw>>.
+Lemma Capability_le_refl: forall r,
+  Capability.le r r.
+Proof. econs; econs 2; econs. Qed.
 
 Lemma fulfill_unset_promises
-      loc from ts msg
+      loc from ts val rel
       promises1 promises2
       l t f m
-      (FULFILL: Memory.fulfill promises1 loc from ts msg promises2)
+      (FULFILL: Memory.remove promises1 loc from ts val rel promises2)
       (TH1: Memory.get l t promises1 = Some (f, m))
       (TH2: Memory.get l t promises2 = None):
-  l = loc /\ t = ts /\ f = from /\ m = msg.
+  l = loc /\ t = ts /\ f = from /\ m.(Message.val) = val /\ Capability.le rel m.(Message.released).
 Proof.
-  exploit Memory.remove_get1; try apply FULFILL; eauto. i. des; [|congr].
-  subst. auto.
+  eapply Memory.remove_get1 in FULFILL; eauto.
+  des; subst.
+  - splits; eauto using Capability_le_refl.
+  - by rewrite TH2 in FULFILL.
 Qed.
 
 Lemma ordering_relaxed_dec
@@ -273,162 +392,369 @@ Proof.
     exploit Memory.promise_promises_get1; eauto. i. des. congr.
   }
   inv STEP0; ss; try by inv LOCAL; ss; congr.
-  - inv LOCAL.
-    + inv FULFILL. ss.
-      exploit fulfill_unset_promises; eauto. i. des. subst.
-      eexists _, _. splits; eauto; ss.
-      destruct (ordering_relaxed_dec ord); auto.
-      unfold Memory.get in TH1. rewrite RELEASE, Cell.bot_get in TH1; auto. congr.
-    + inv PROMISE.
-      exploit Memory.promise_promises_get1; eauto. i. des.
-      inv FULFILL. ss.
-      exploit fulfill_unset_promises; eauto. i. des. subst.
-      eexists _, _. splits; eauto; ss.
-      destruct (ordering_relaxed_dec ord); auto.
-      unfold Memory.get in TH1. rewrite RELEASE, Cell.bot_get in TH1; auto. congr.
-  - inv LOCAL1. inv LOCAL2.
-    + inv FULFILL. ss.
-      exploit fulfill_unset_promises; eauto. i. des. subst.
-      eexists _, _. splits; eauto; ss.
-      destruct (ordering_relaxed_dec ordw); auto.
-      unfold Memory.get in TH1. rewrite RELEASE, Cell.bot_get in TH1; auto. congr.
-    + inv PROMISE.
-      exploit Memory.promise_promises_get1; eauto. i. des.
-      inv FULFILL. ss.
-      exploit fulfill_unset_promises; eauto. i. des. subst.
-      eexists _, _. splits; eauto; ss.
-      destruct (ordering_relaxed_dec ordw); auto.
-      unfold Memory.get in TH1. rewrite RELEASE, Cell.bot_get in TH1; auto. congr.
+  - by rewrite TH1 in TH2.
+  - inv LOCAL. inv WRITE.
+    exploit Memory.promise_promises_get1; eauto. i. des.
+    exploit fulfill_unset_promises; eauto. i. des. subst.
+    esplits; eauto; s; eauto.
+    destruct (ordering_relaxed_dec ord); auto.
+    apply RELEASE in H. des. unfold Memory.get in *.
+    by ss; rewrite H, Cell.bot_get in TH1.
+  - inv LOCAL1. inv LOCAL2. inv WRITE.
+    exploit Memory.promise_promises_get1; eauto. i. des.
+    exploit fulfill_unset_promises; eauto. i. des. subst.
+    esplits; eauto; s; eauto.
+    destruct (ordering_relaxed_dec ordw); auto.
+    apply RELEASE in H. des. unfold Memory.get in *.
+    by ss; rewrite H, Cell.bot_get in TH1.
 Qed.
 
 Lemma pi_steps_promise
       tid
-      c1 lang1 st1 lc1
-      c3 lang3 st3 lc3
+      cST1 lst1 lc1
+      cST3 lst3 lc3
       loc from ts msg
-      (WF1: Configuration.wf c1)
-      (STEPS: rtc (pi_step tid) c1 c3)
-      (TH1: IdentMap.find tid c1.(Configuration.threads) = Some (existT _ lang1 st1, lc1))
-      (TH3: IdentMap.find tid c3.(Configuration.threads) = Some (existT _ lang3 st3, lc3))
+      (WF1: pi_wf cST1)
+      (STEPS: rtc (pi_step tid) cST1 cST3)
+      (TH1: IdentMap.find tid cST1.(snd).(Configuration.threads) = Some (lst1, lc1))
+      (TH3: IdentMap.find tid cST3.(snd).(Configuration.threads) = Some (lst3, lc3))
       (GET1: Memory.get loc ts lc1.(Local.promises) = Some (from, msg))
       (GET3: Memory.get loc ts lc3.(Local.promises) = None):
-  exists c2 lang2 st2 lc2 e2 st2' ord2,
-    <<STEPS: rtc (pi_step tid) c1 c2>> /\
-    <<TH2: IdentMap.find tid c2.(Configuration.threads) = Some (existT _ lang2 st2, lc2)>> /\
+  exists cST2 lang2 st2 lc2 e2 st2' ord2,
+    <<STEPS: rtc (pi_step tid) cST1 cST2>> /\
+    <<TH2: IdentMap.find tid cST2.(snd).(Configuration.threads) = Some (existT _ lang2 st2, lc2)>> /\
     <<STATE2: lang2.(Language.step) (Some e2) st2 st2'>> /\
     <<EVENT2: ProgramEvent.is_writing e2 = Some (loc, ord2)>> /\
     <<ORD2: Ordering.le ord2 Ordering.relaxed>>.
 Proof.
-  revert lang1 st1 lc1 from msg TH1 GET1.
+  revert lst1 lc1 from msg TH1 GET1.
   induction STEPS; i.
-  { rewrite TH1 in TH3. inv TH3. apply inj_pair2 in H1. congr. }
-  inversion H. inv STEP. destruct (Memory.get loc ts lc2.(Local.promises)) as [[]|] eqn:X.
+  { rewrite TH1 in TH3. inv TH3. rewrite GET3 in GET1. done. }
+  inversion H. subst. inv STEPT. destruct (Memory.get loc ts lc2.(Local.promises)) as [[]|] eqn:X.
   { exploit IHSTEPS; eauto; s.
-    { inv H. eapply small_step_future; eauto. }
+    { eapply pi_step_future; cycle 1; eauto. }
     { rewrite IdentMap.Facts.add_eq_o; eauto. }
-    i. des. eexists _, _, _, _, _, _, _. splits; [|eauto|eauto|eauto|eauto].
+    i. des. esplits; cycle 1; eauto.
     etrans; [|eauto]. econs 2; [|econs 1]. eauto.
   }
-  clear H STEPS IHSTEPS. rewrite TH1 in TID. inv TID. apply inj_pair2 in H1. subst.
+  clear H STEPS IHSTEPS. ss. rewrite TH1 in TID. inv TID. 
   exploit thread_step_unset_promises; eauto; s.
-  { eapply WF1. eauto. }
-  i. des. eexists _, _, _, _, _, _, _. splits; eauto.
+  { inv WF1. s. eapply WFT. eauto. }
+  i. des. inv WF1. esplits; eauto.
 Qed.
 
-Lemma pi_consistent_small_step_pi
-      e tid c1 c2 c3
-      (PI_CONSISTENT: pi_consistent c1)
-      (WF: Configuration.wf c1)
-      (CONSISTENT: Configuration.consistent c1)
-      (PI_RACEFREE: pi_racefree c1)
-      (PI_STEPS: rtc (pi_step tid) c1 c2)
-      (STEP: small_step e tid c2 c3):
-  pi_machine_event e c2.(Configuration.threads).
+Hint Constructors small_step.
+Hint Constructors Thread.program_step.
+Hint Constructors Thread.step.
+
+Lemma race_pi_wf
+      cST ord1 ord2
+      (WF: pi_wf cST)
+      (RACE: race (snd cST) ord1 ord2):
+  race (fst cST) ord1 ord2.
 Proof.
-  unfold pi_machine_event. destruct (ThreadEvent.is_reading e) as [[[]]|] eqn:E; auto. ii.
-  inv H.
-  assert (tid <> tid0).
-  { admit. (* consistency required *) }
-  exploit PI_CONSISTENT.
-  { erewrite <- rtc_pi_step_find; eauto. congr. }
-  { eapply rtc_implies; try apply PI_STEPS; eauto.
-    i. econs; eauto.
-  }
+  inv WF. inv RACE.
+  ss. econs; cycle 3; [apply STATE1|apply STATE2|..]; eauto. 
+  - s. setoid_rewrite IdentMap.Properties.F.map_o. by rewrite TH1.
+  - s. setoid_rewrite IdentMap.Properties.F.map_o. by rewrite TH2.
+Qed.
+
+Lemma consistent_small_step_pi
+      e tid c1 c2 c3
+      (CONSISTENT: Configuration.consistent c1)
+      (STEPS: rtc (small_step_all tid) c1 c2)
+      (STEP: small_step e tid c2 c3):
+   forall loc to ord
+     (RW: ThreadEvent.is_reading e = Some (loc, to, ord)),
+  ~Threads.is_promised tid loc to c2.(Configuration.threads).
+Proof.
+Admitted.
+
+Lemma pi_steps_small_steps_t
+      tid cST1 cST2
+      (PI_STEPS: rtc (pi_step tid) cST1 cST2):
+  rtc (small_step_all tid) (snd cST1) (snd cST2).
+Proof.
+  apply Operators_Properties.clos_rt_rt1n_iff in PI_STEPS.
+  induction PI_STEPS; eauto.
+  - econs; eauto. inv H. econs; eauto.
+  - etransitivity; eauto.
+Qed.
+
+Lemma pi_consistent_small_step_pi_rw
+      e tid cST1 cST2 cT3
+      (WF: pi_wf cST1)
+      (PI_CONSISTENT: pi_consistent cST1)
+      (CONSISTENT: Configuration.consistent cST1.(snd))
+      (PI_RACEFREE: pi_racefree cST1)
+      (PI_STEPS: rtc (pi_step tid) cST1 cST2)
+      (STEP: small_step e tid cST2.(snd) cT3):
+  forall loc to ord tid' ts
+    (NEQ: tid <> tid')
+    (RW: ThreadEvent.is_reading e = Some (loc, to, ord) \/
+         ThreadEvent.is_writing e = Some (loc, to, ord)),
+  ~Threads.is_promised tid' loc ts cST2.(snd).(Configuration.threads).
+Proof.
+  ii. inv H.
+  inv PI_CONSISTENT. ss.
+  guardH RW. destruct cST2 as [cS2 cT2].
+  exploit CONSIS.
+  { eapply rtc_implies, PI_STEPS. i. econs; eauto. }
+  { eauto. }
+  { eauto. }
   i. des.
-  exploit pi_steps_promise.
-  { eapply rtc_pi_step_future; eauto. }
-  { eauto. }
-  { eauto. }
-  { eauto. }
-  { eauto. }
-  { rewrite PROMISES0. apply Memory.bot_get. }
-  i. des.
-  exploit PI_RACEFREE.
+  exploit pi_steps_promise; try apply PROMISE; [eapply rtc_pi_step_future|..]; eauto.
+  i; des.
+  exploit (PI_RACEFREE cST2 ord ord2).
   { etrans.
-    - eapply rtc_implies; try apply PI_STEPS; eauto.
+    - eapply rtc_implies, PI_STEPS; eauto.
       i. econs. eauto.
-    - eapply rtc_implies; try apply STEPS0; eauto.
+    - eapply rtc_implies, STEPS0.
       i. econs. eauto.
   }
   { (* TODO: is ThreadEvent.is_reading/writing neccessary? *)
-    inv STEP. inv STEP0; [by inv E|].
+    inv STEP. inv STEP0; [by inv STEP; inv RW; inv H|].
     erewrite <- rtc_pi_step_find in TID0; eauto.
-    inv STEP; inv E.
-    - econs; eauto; ss.
-    - econs; eauto; ss.
+    apply race_pi_wf. 
+    { eapply rtc_pi_step_future, STEPS0. 
+      by eapply rtc_pi_step_future; eauto. }
+    inv STEP; inv RW; inv H
+    ; econs; eauto; first [by econs 1; ss|by econs 2; ss].
   }
-  i. des. destruct ord2; inv x0; inv x1.
+  i. des. by destruct ord2; inv x0; inv x1.
+Qed.
+
+Lemma pi_consistent_small_step_pi
+      e tid cST1 cST2 cT3
+      (WF: pi_wf cST1)
+      (PI_CONSISTENT: pi_consistent cST1)
+      (CONSISTENT: Configuration.consistent cST1.(snd))
+      (PI_RACEFREE: pi_racefree cST1)
+      (PI_STEPS: rtc (pi_step tid) cST1 cST2)
+      (STEP: small_step e tid cST2.(snd) cT3):
+  exists cS3, pi_step tid cST2 (cS3,cT3).
+Proof.
+  destruct cST1 as [cS1 cT1], cST2 as [cS2 cT2].
+  assert (RW:= pi_consistent_small_step_pi_rw WF PI_CONSISTENT CONSISTENT PI_RACEFREE PI_STEPS STEP).
+  assert (R:= consistent_small_step_pi CONSISTENT (pi_steps_small_steps_t PI_STEPS) STEP).
+  exploit rtc_pi_step_future; eauto. 
+  i; des. inv WF2. ss. inv STEP. inv STEP0.
+  - eexists. econs; [by eauto|by inv STEP; s; eauto|].
+    inv STEP. ss. rewrite IdentMap.gss.
+    setoid_rewrite IdentMap.Properties.F.map_o.
+    by rewrite TID.
+  - inv STEP.
+    { eexists. econs.
+      - econs; eauto.
+      - econs.
+        + ss. setoid_rewrite IdentMap.Properties.F.map_o.
+          by rewrite TID. 
+        + econs 2; econs 1; eauto.
+      - s. by rewrite !IdentMap.gss.
+    }
+    { inv LOCAL. eexists. econs.
+      - econs; eauto. econs 2. econs 2; eauto. econs; eauto.
+      - econs.
+        + ss. setoid_rewrite IdentMap.Properties.F.map_o.
+          by rewrite TID. 
+        + econs 2; econs 2; eauto.
+          econs; eauto.
+          s. eapply RL; eauto.
+          i. destruct (Ident.eq_dec tid tid0) eqn: EQ.
+          * subst. eapply R; s; eauto.
+          * eapply RW; s; eauto.
+      - s. by rewrite !IdentMap.gss.
+    }
+    { inv LOCAL. inv WRITE. eexists. econs.
+      - econs; eauto. econs 2. econs 3; eauto. econs; eauto. econs; eauto.
+      - econs.
+        + ss. setoid_rewrite IdentMap.Properties.F.map_o.
+          by rewrite TID. 
+        + econs 2; econs 3; eauto. 
+          econs; [|by esplits; [|apply RELEASE]].
+          admit.
+      - s. by rewrite !IdentMap.gss.
+    }
+    { admit.
+    }
+    { inv LOCAL. eexists. econs.
+      - econs; eauto. econs 2. econs 5; eauto. econs; eauto.
+      - econs.
+        + ss. setoid_rewrite IdentMap.Properties.F.map_o.
+          by rewrite TID. 
+        + econs 2; econs 5; eauto.
+          econs; eauto.
+      - s. by rewrite !IdentMap.gss.
+    }
+    { inv LOCAL. eexists. econs.
+      - econs; eauto. econs 2. econs 6; eauto. econs; eauto.
+      - econs.
+        + ss. setoid_rewrite IdentMap.Properties.F.map_o.
+          by rewrite TID. 
+        + econs 2; econs 6; eauto.
+          econs; eauto.
+      - s. by rewrite !IdentMap.gss.
+    }
 Admitted.
 
 Lemma pi_consistent_rtc_tau_small_step_pi
-      tid c1 c2 c3
-      (PI_CONSISTENT: pi_consistent c1)
-      (WF: Configuration.wf c1)
-      (CONSISTENT: Configuration.consistent c1)
-      (PI_RACEFREE: pi_racefree c1)
-      (PI_STEPS: rtc (pi_step tid) c1 c2)
-      (STEP: rtc (tau_small_step tid) c2 c3):
-  rtc (pi_step tid) c2 c3.
+      tid cST1 cST2 cT3
+      (WF: pi_wf cST1)
+      (PI_CONSISTENT: pi_consistent cST1)
+      (CONSISTENT: Configuration.consistent cST1.(snd))
+      (PI_RACEFREE: pi_racefree cST1)
+      (PI_STEPS: rtc (pi_step tid) cST1 cST2)
+      (STEP: rtc (tau_small_step tid) cST2.(snd) cT3):
+  exists cS3, rtc (pi_step tid) cST2 (cS3,cT3).
 Proof.
   apply Operators_Properties.clos_rt_rt1n_iff in STEP.
   apply Operators_Properties.clos_rt_rtn1_iff in STEP.
-  induction STEP; auto. etrans; eauto. econs 2; [|econs 1].
-  inv H. econs; eauto. eapply pi_consistent_small_step_pi; eauto.
-  etrans; eauto.
+  destruct cST2 as [cS2 cT2].
+  induction STEP; eauto.
+  des. inv H. ss.
+  exploit pi_consistent_small_step_pi; try etransitivity; eauto.
+  i; des. eexists. etrans; eauto. econs; eauto.
 Qed.
 
 Lemma pi_consistent_step_pi
-      c1 c2
-      e tid
-      (PI_CONSISTENT: pi_consistent c1)
-      (WF: Configuration.wf c1)
-      (CONSISTENT: Configuration.consistent c1)
-      (PI_RACEFREE: pi_racefree c1)
-      (STEP: Configuration.step e tid c1 c2):
-  rtc (pi_step tid) c1 c2.
+      cST1 cT2 e tid
+      (WF: pi_wf cST1)
+      (PI_CONSISTENT: pi_consistent cST1)
+      (CONSISTENT: Configuration.consistent cST1.(snd))
+      (PI_RACEFREE: pi_racefree cST1)
+      (STEP: Configuration.step e tid cST1.(snd) cT2):
+  exists cS2, rtc (pi_step tid) cST1 (cS2,cT2).
 Proof.
-  exploit step_small_steps; eauto. i. des. subst.
-  exploit pi_consistent_rtc_tau_small_step_pi; eauto. i.
-  exploit pi_consistent_small_step_pi; eauto. i.
-  etrans; eauto. econs 2; [|econs 1]. econs; eauto.
+  exploit step_small_steps; eauto; [by inv WF|].
+  i. des. subst.
+  exploit pi_consistent_rtc_tau_small_step_pi; eauto. i; des.
+  exploit pi_consistent_small_step_pi; eauto. i; des.
+  eexists. etrans; eauto. econs; eauto.
 Qed.
 
-Lemma pi_consistent_pi_step_pi_consistent
-      c1 c2
-      tid
-      (PI_CONSISTENT: pi_consistent c1)
-      (WF1: Configuration.wf c1)
-      (WF2: Configuration.wf c2)
-      (CONSISTENT1: Configuration.consistent c1)
-      (CONSISTENT2: Configuration.consistent c2)
-      (STEP: rtc (pi_step tid) c1 c2):
-  pi_consistent c2.
-Proof.
-  ii. destruct (Ident.eq_dec tid tid0).
-  - subst tid0.
-    (* TODO: sketch the proof *)
-    admit.
-  - eapply PI_CONSISTENT.
-    + erewrite <- rtc_pi_step_find; eauto.
-    + etrans; [|eauto]. eapply rtc_implies; [|apply STEP]. econs; eauto.
-Admitted.
+
+
+
+
+
+
+
+
+
+
+
+
+
+
+
+
+(* Lemma pi_consistent_pi_step_pi_consistent *)
+(*       c1 c2 *)
+(*       tid *)
+(*       (PI_CONSISTENT: pi_consistent c1) *)
+(*       (PI_RACEFREE: pi_racefree c1) *)
+(*       (WF1: Configuration.wf c1) *)
+(*       (WF2: Configuration.wf c2) *)
+(*       (CONSISTENT1: Configuration.consistent c1) *)
+(*       (CONSISTENT2: Configuration.consistent c2) *)
+(*       (STEP: rtc (pi_step tid) c1 c2): *)
+(*   pi_consistent c2. *)
+(* Proof. *)
+(*   ii. destruct (Ident.eq_dec tid tid0). *)
+(*   - subst tid0. *)
+(*     (* TODO: sketch the proof *) *)
+(*     admit. *)
+(*   - eapply PI_CONSISTENT. *)
+(*     + erewrite <- rtc_pi_step_find; eauto. *)
+(*     + etrans; [|eauto]. eapply rtc_implies; [|apply STEP]. econs; eauto. *)
+(* Admitted. *)
+
+
+(* Lemma memory_lower_get1: *)
+(*   forall mem1 mem2 loc from ts val rel1 rel2 l t f v r1 *)
+(*      (MEM: Memory.lower mem1 loc from ts val rel1 rel2 mem2) *)
+(*      (GET: Memory.get l t mem1 = Some (f, Message.mk v r1)), *)
+(*   exists r2, Memory.get l t mem2 = Some (f, Message.mk v r2) /\  *)
+(*   Capability.le r2 r1. *)
+(* Proof. *)
+(*   i. inv MEM. inv REMOVE. inv ADD. *)
+(*   unfold Memory.get in *.  *)
+(*   destruct (Loc.eq_dec l loc); subst. *)
+(*   - setoid_rewrite LocFun.add_spec_eq in ADD0. *)
+(*     setoid_rewrite LocFun.add_spec_eq. *)
+(*     inv REMOVE0. destruct (Time.eq_dec t ts); subst. *)
+(*     + setoid_rewrite GET in GET0. inv GET0. *)
+(*       esplits; eauto. *)
+(*       setoid_rewrite Cell.add_get2; eauto. *)
+(*     + inv ADD0. unfold Cell.get. rewrite <-H1. *)
+(*       rewrite DenseOrder.DOMap.gso; eauto. *)
+(*       rewrite <- H0, DenseOrder.DOMap.gro; eauto. *)
+(*       esplits; eauto using Capability_le_refl. *)
+(*   - setoid_rewrite LocFun.add_spec_neq; eauto. *)
+(*     setoid_rewrite LocFun.add_spec_neq; eauto. *)
+(*     esplits; eauto using Capability_le_refl. *)
+(* Qed.     *)
+
+
+(* Inductive pf_rel: Configuration.t -> Configuration.t -> Prop := *)
+(* | pf_rel_base  *)
+(*     c *)
+(*     (PRBOT: forall tid lang st lc *)
+(*               (TH: IdentMap.find tid c.(Configuration.threads) = Some (existT _ lang st, lc)), *)
+(*             lc.(Local.promises) = Memory.bot):  *)
+(*   pf_rel c c *)
+
+(* | pf_rel_promise *)
+(*     e tid cS cT cT' *)
+(*     (REL: pf_rel cS cT) *)
+(*     (STEPT: small_step e tid cT cT') *)
+(*     (PROMISE: match e with | ThreadEvent.promise _ _ _ _ _ => True | _ => False end): *)
+(*   pf_rel cS cT' *)
+
+(* | pf_rel_other *)
+(*     e tid cS cS' cT cT' *)
+(*     (REL: pf_rel cS cT) *)
+(*     (STEPS: small_step e tid cS cS') *)
+(*     (STEPT: small_step e tid cT cT') *)
+(*     (PROMISE: match e with | ThreadEvent.promise _ _ _ _ _ => False | _ => True end): *)
+(*   pf_rel cS cT' *)
+(* . *)
+
+(* Definition pi_machine_event (e:ThreadEvent.t) tid (threads:Threads.t): Prop := *)
+(*   forall loc to ord ts tid' *)
+(*     (RW: ThreadEvent.is_reading e = Some (loc, to, ord) \/ *)
+(*          ThreadEvent.is_writing e = Some (loc, to, ord)) *)
+(*     (TNEQ: tid <> tid'), *)
+(*   ~ Threads.is_promised tid' loc ts threads. *)
+
+(* Inductive pi_step (tid:Ident.t) (c1 c2:Configuration.t): Prop := *)
+(* | pi_step_intro *)
+(*     e *)
+(*     (STEP: small_step e tid c1 c2) *)
+(*     (READINFO: pi_machine_event e tid c1.(Configuration.threads)) *)
+(* . *)
+
+(* Inductive pi_step_all (c1 c2:Configuration.t): Prop := *)
+(* | pi_step_all_intro *)
+(*     tid *)
+(*     (PI_STEP: pi_step tid c1 c2) *)
+(* . *)
+
+(* Inductive pi_step_except (tid_except:Ident.t) (c1 c2:Configuration.t): Prop := *)
+(* | pi_step_except_intro *)
+(*     tid *)
+(*     (PI_STEP: pi_step tid c1 c2) *)
+(*     (TID: tid <> tid_except) *)
+(* . *)
+
+(* Definition pi_consistent (c1:Configuration.t): Prop := *)
+(*   forall tid lang c2 st2 lc2 loc ts from msg *)
+(*     (TID: IdentMap.find tid c1.(Configuration.threads) <> None) *)
+(*     (STEPS: rtc (pi_step_except tid) c1 c2) *)
+(*     (THREAD: IdentMap.find tid c2.(Configuration.threads) = Some (existT _ lang st2, lc2)) *)
+(*     (PROMISE: Memory.get loc ts lc2.(Local.promises) = Some (from, msg)), *)
+(*   exists c3 st3 lc3, *)
+(*     <<STEPS: rtc (pi_step tid) c2 c3>> /\ *)
+(*     <<THREAD: IdentMap.find tid c3.(Configuration.threads) = Some (existT _ lang st3, lc3)>> /\ *)
+(*     <<PROMISE: Memory.get loc ts lc3.(Local.promises) = None>>. *)
+
