src/lang/Configuration.v
@@ -84,9 +84,9 @@ Module Threads.
     IdentMap.find tid (compose ths1 ths2) = compose_option (IdentMap.find tid ths1) (IdentMap.find tid ths2).
   Proof. apply IdentMap.Facts.map2_1bis; auto. Qed.
 
-  Inductive is_promised (loc:Loc.t) (to:Time.t) (threads:t): Prop :=
+  Inductive is_promised tid (loc:Loc.t) (to:Time.t) (threads:t): Prop :=
   | is_promised_intro
-      tid lang st lc from msg
+      lang st lc from msg
       (TID: IdentMap.find tid threads = Some (existT _ lang st, lc))
       (PROMISES: Memory.get loc to lc.(Local.promises) = Some (from, msg))
   .
